% JUMP TO LINE 60, 73
\documentclass[preview, margin=0.6in]{standalone}
\usepackage[letterpaper,portrait,top=0.4in, left=0.6in, right=0.6in, bottom=1in]{geometry}

\usepackage{amsmath, amsfonts, amsthm, amssymb}
\usepackage{graphicx, float}
\usepackage{mathtools}
\usepackage{titlesec}
\usepackage{interval}
\usepackage{hyperref}
\usepackage{siunitx}
\usepackage{titling}
\usepackage{vwcol}
\usepackage{setspace}
\usepackage{empheq}
\usepackage{cancel}
\usepackage{esdiff}
\usepackage{multicol}
\usepackage{mdframed}
\usepackage{esdiff}
\usepackage{tikzsymbols}
\usepackage{multicol}
\usepackage{tikz}
\usepackage{varwidth}
\usepackage{pgfplots}
\pgfplotsset{compat=1.18}
\intervalconfig {
	soft open fences
}

\newcommand{\alignedintertext}[1]{%
  \noalign{%
    \vskip\belowdisplayshortskip
    \vtop{\hsize=\linewidth#1\par
    \expandafter}%
    \expandafter\prevdepth\the\prevdepth
  }%
}

\newtheorem{lemma}{Lemma}

\renewcommand{\qedsymbol}{\Smiley[1.3]}
\newcommand*{\problem}[1]{\section*{Problem #1}}
\newcommand*{\aps}{\section*{AP Corner}}
\newcommand*{\deriv}[1][x]{\ensuremath{\dfrac{\mathrm{d}}{\mathrm{d}#1}}}
\newcommand*{\floor}[1]{\ensuremath{\lfloor #1\rfloor}}
\newcommand*{\lheqzero}{\ensuremath{\underset{\text{L'H}}{\overset{\left[\frac00\right]}{=}}}}
\newcommand*{\lheqinfty}{\ensuremath{\underset{\text{L'H}}{\overset{\left[\frac{\infty}{\infty}\right]}{=}}}}

\DeclareMathOperator{\DNE}{DNE}
\DeclareMathOperator{\sgn}{sgn}

\DeclareMathOperator{\arccsc}{arccsc}
\DeclareMathOperator{\arcsec}{arcsec}
\DeclareMathOperator{\arccot}{arccot}

\setlength{\parindent}{0pt}

%opening
\title{\vspace*{-30pt}Problem Set \#15}
\author{Jayden Li}
\date{\today}

% \allowdisplaybreaks
\postdisplaypenalty=100000

\begin{document}
\setstretch{1.25}
\fontsize{12pt}{12pt}\selectfont
\setlength{\abovedisplayskip}{0pt}
\maketitle
\problem{1}
\begin{itemize}
	\item[(a)]
		$\begin{aligned}[t]
		    \int \cos \sqrt{x}\,\mathrm{d}x
			&=\int 2\sqrt{x}\cos\left(\sqrt{x}\right)\frac{1}{2 \sqrt{x}}\,\mathrm{d}x
			=\left[\begin{aligned}
			    t&=\sqrt{x} \\
				\mathrm{d}t&=\frac{\mathrm{d}x}{2 \sqrt{x}}
			\end{aligned}\right]
			2 \int t\cos t\,\mathrm{d}t \\
			&=\left[\begin{alignedat}{2}
					u&=t &\quad \mathrm{d}u&=\mathrm{d}t \\
					\mathrm{d}v&=\cos t \,\mathrm{d}t & v&=\sin t
			\end{alignedat}\right]
			2\left(t\sin t-\int \sin t\,\mathrm{d}t\right) \\
			&=2t\sin t-2(-\cos t)
			=\boxed{2\sqrt{x}\sin\left(\sqrt{x}\right)+2\cos \sqrt{x}+C}
		\end{aligned}$
\end{itemize}

\problem{2}
\begin{itemize}
	\item[(a)]
		$\begin{aligned}[t]
		    \int (2x+3)e^x\,\mathrm{d}x
			&=\left[\begin{alignedat}{2}
					u&=2x+3 &\quad \mathrm{d}u&=2 \,\mathrm{d}x \\
					\mathrm{d}v&=e^x \,\mathrm{d}x & v&=e^x
			\end{alignedat}\right]
			(2x+3)e^x-2 \int e^x\,\mathrm{d}x
			=\boxed{2xe^x+e^x+C}
		\end{aligned}$
\end{itemize}

\problem{4}
\begin{itemize}
	\item[(a)]
		$\begin{aligned}[t]
		    \int \sin^2x\,\mathrm{d}x
			&=-\frac12 \cos (x) \sin^{2-1}(x)+\frac{2-1}{2}\int \sin^{2-2}(x)\,\mathrm{d}x
			=-\frac14\cdot2\cos(x)\sin(x)+\frac12 \int 1\,\mathrm{d}x \\
			&=\frac x2-\frac{\sin2x}{4}+C
		\end{aligned}$

	\item[(b)]
		$\begin{aligned}[t]
		    \int \sin^4x\,\mathrm{d}x
			&=-\frac14 \cos (x) \sin^{4-1}(x)+\frac{4-1}{4}\int \sin^{4-2}(x)\,\mathrm{d}x
			=-\frac14\cos(x)\sin^3(x)+\frac34 \int \sin^2(x)\,\mathrm{d}x \\
			&=-\frac{\sin2x}{8}\cdot\sin^2x+\frac34\left(\frac x2-\frac{\sin 2x}{4}\right)
			=-\frac{2\sin2x}{16}\cdot\sin^2x+\frac{3x}{8}-\frac{3\sin 2x}{16} \\
			&=\boxed{\frac{\sin2x}{16}\left(-2\sin^2x-3\right)+\frac{3x}{8}+C}
		\end{aligned}$
\end{itemize}

\problem{6}
\begin{itemize}
	\item[(b)]
		$\begin{aligned}[t]
			\int \left(\tan^n x+\tan^{n-2}x\right)\,\mathrm{d}x
			&=\left[\begin{alignedat}{2}
					u&=\tan^{n-2}x &\quad \mathrm{d}u&=(n-2)\tan^{n-3}(x)\sec^2(x)\,\mathrm{d}x \\
					\mathrm{d}v&=\left(\tan^2(x)+1\right)\,\mathrm{d}x & v&=\tan x
			\end{alignedat}\right] \\
			&\phantom{={}}\tan^{n-2}(x)\tan(x)-(n-2)\int \tan^{n-3}(x)\tan(x)\sec^2(x)\,\mathrm{d}x \\
			\int \tan^nx\,\mathrm{d}x+\int \tan^{n-2}x\,\mathrm{d}x&=\tan^{n-1}x-(n-2)\int \tan^{n-2}(x)\sec^2(x)\,\mathrm{d}x \\
			&=\left[\begin{aligned}
				t&=\tan x \\
				\mathrm{d}t&=\sec^2(x)\,\mathrm{d}x
			\end{aligned}\right]
			\tan^{n-1}x-(n-2)\int t^{n-2}\,\mathrm{d}t \\
			\int \tan^nx\,\mathrm{d}x&=\tan^{n-1}x-\frac{(n-2)t^{n-1}}{n-1}-\int \tan^{n-2}x\,\mathrm{d}x \\
			&=\frac{(n-1)\tan^{n-1}x-(n-2)\tan^{n-1}x}{n-1}-\int \tan^{n-2}x\,\mathrm{d}x \\
			&=\frac{\cancel{n\tan^{n-1}x}-\tan^{n-1}x-\cancel{n\tan^{n-1}x}+2\tan^{n-1}x}{n-1}-\int \tan^{n-2}x\,\mathrm{d}x \\
			\Aboxed{\int \tan^nx\,\mathrm{d}x&=\frac{\tan^{n-1}x}{n-1}-\int \tan^{n-2}\,\mathrm{d}x}
		\end{aligned}$
\end{itemize}

\problem{7}
$\begin{aligned}[t]
	\text{Distance traveled}
	&=\int_{0}^{t}x^2e^{-x}\mathrm{d}x
	=\left[\begin{alignedat}{2}
			u_1&=x^2 &\quad \mathrm{d}u_1&=2x \,\mathrm{d}x \\
			\mathrm{d}v_1&=e^{-x}\,\mathrm{d}x & v_1&=-e^{-x}
	\end{alignedat}\right] 
	\left[-x^2e^{-x}\right]_{0}^{t}+2\int_{0}^{t}xe^{-x}\,\mathrm{d}x \\
	&=\left[\begin{alignedat}{2}
			u_2&=x &\quad \mathrm{d}u_2&=\mathrm{d}x \\
			\mathrm{d}v_2&=e^{-x}\,\mathrm{d}x & v_2&=-e^{-x}
	\end{alignedat}\right] 
	-t^2e^{-t}+2 \left[-xe^{-x}\right]_{0}^{t}+2 \int_{0}^{t}e^{-x}\,\mathrm{d}x \\
	&=-t^2e^{-t}-2te^{-t}+2 \left[-e^{-x}\right]_{0}^{t}
	=-t^2e^{-t}-2te^{-t}+2\left(-e^{-t}-(-1)\right) \\
	&=\boxed{-t^2e^{-t}-2te^{-t}-2e^{-t}+2}
\end{aligned}$

\problem{8}
$\begin{aligned}[t]
    \int_{1}^{4}xf''(x)\,\mathrm{d}x
	&=\left[\begin{alignedat}{2}
			u&=x &\quad \mathrm{d}u&=\mathrm{d}x \\
			\mathrm{d}v&=f''(x)\,\mathrm{d}x & v&=f'(x)
	\end{alignedat}\right] 
	\left[xf'(x)\right]_{1}^{4}-\int_{1}^{4}f'(x)\,\mathrm{d}x
	=4f'(4)-f'(1)-\left[f(x)\right]_{1}^{4} \\
	&=4\cdot3-5-f(4)+f(1)
	=12-5-7+2
	=\boxed{2}
\end{aligned}$

\end{document}
