\documentclass{article}

\usepackage[letterpaper,portrait,top=0.4in, left=0.8in, right=0.8in, bottom=1in]{geometry}

\usepackage{amsmath, amsfonts, amsthm, amssymb}
\usepackage{graphicx, float}
\usepackage{mathtools}
\usepackage{titlesec}
\usepackage{interval}
\usepackage{titling}
\usepackage{vwcol}
\usepackage{empheq}
\usepackage{cancel}

\intervalconfig {
	soft open fences
}

\newcommand{\alignedintertext}[1]{%
	\noalign{%
		\vskip\belowdisplayshortskip
		\vtop{\hsize=\linewidth#1\par
		\expandafter}%
		\expandafter\prevdepth\the\prevdepth
	}%
}

\allowdisplaybreaks

%opening
\title{Finish Problem Set \#42}
\author{Jayden Li}
\date{January 17, 2024}

\begin{document}

\newgeometry{top=0.4in, left=0.6in, right=0.6in, bottom=1in}

\fontsize{12pt}{12pt}\selectfont

\maketitle

\section*{Problem 6}
\begin{itemize}
\item[(b)]
\begin{align*}
	1^3+2^3+3^3+\cdots+n^3&\stackrel{?}{=}(1+2+3+\cdots+n)^2 \\
	\sum_{k=1}^{n}k^3&\stackrel{?}{=}\left(\sum_{k=1}^{n}k\right)^2
\end{align*}
\begin{proof}
	By induction. \\ \\
	\textbf{Base case.} $n=1$ \\
	\begin{minipage}[t]{0.2\linewidth}
		LHS: $\displaystyle \sum_{k=1}^{1}k^3=1$
	\end{minipage}
	\begin{minipage}[t]{0.3\linewidth}
		RHS: $\displaystyle \left(\sum_{k=1}^{1}k\right)^2=1$
	\end{minipage}
	\\
	\textbf{Induction Hypothesis.} Suppose $\displaystyle
	\sum_{k=1}^{n}k^3=\left(\sum_{k=1}^{n}k\right)^2$. Show
	$\displaystyle \sum_{k=1}^{n+1}k^3=\left(\sum_{k=1}^{n+1}k
	\right)^2$
	\\
	\textbf{Inductive Step.}
	$\begin{aligned}[t]
		\left(\sum_{k=1}^{n+1}k\right)^2
		&=\left(\sum_{k=1}^{n}k+(n+1)\right)^2 \\
		&=\left(\sum_{k=1}^{n}k\right)^2+
			2\left(\sum_{k=1}^{n}k\right)(n+1)+(n+1)^2 \\
		&=\sum_{k=1}^{n}k^3+2\left(\frac{n(n+1)(n+1)}{2}\right)+
			(n+1)^2 \\
		&=\frac{n^2(n+1)^2}{4}+\frac{4n(n+1)^2}{4}+\frac{4(n+1)^2}{n} \\
		&=\frac{(n+1)^2\left(n^2+4n+4\right)}{4} \\
		&=\frac{(n+1)^2(n+2)^2}{4} \\
		&=\sum_{k=1}^{n+1}k^3
	\end{aligned}$ \\
\end{proof}

\section*{Problem 7}
\setlength{\abovedisplayskip}{0pt}
\begin{align*}
	\sum_{i=1}^{4}\sum_{j=1}^{4}(i-j)^2
	&=\sum_{i=1}^{4}\sum_{j=1}^{4}\left(i^2-2ij+j^2\right) \\
	&=\sum_{i=1}^{4}\left(\sum_{j=1}^{4}i^2-2\sum_{j=1}^{4}ij+
		\sum_{j=1}^{4}j^2\right) \\
	&=\sum_{i=1}^{4}\left(4i^2-2i\sum_{j=1}^{4}j+
		\sum_{j=1}^{4}j^2\right) \\
	&=\sum_{i=1}^{4}4i^2-\sum_{i=1}^{4}\left(2i\left(\frac
		{4(4+1)}{2}\right)-\frac{4(4+1)(2(4)+1)}{6}\right) \\
	&=4\left(\frac{4(4+1)(2(4)+1)}{6}\right)-
		\sum_{i=1}^{4}\left(20i-30\right) \\
	&=4\cdot30-20\sum_{i=1}^{4}i+\sum_{i=1}^{4}30 \\
	&=120-20\left(\frac{4(4+1)}{2}\right)+4\cdot30 \\
	&=240-200 \\
	&=\boxed{40}
\end{align*}

\end{itemize}

\end{document}