\documentclass{article}

\usepackage[letterpaper,portrait,top=0.4in, left=0.6in, right=0.6in, bottom=1in]{geometry}

\usepackage{amsmath, amsfonts, amsthm, amssymb}
\usepackage{graphicx, float}
\usepackage{mathtools}
\usepackage{titlesec}
\usepackage{interval}
\usepackage{hyperref}
\usepackage{siunitx}
\usepackage{titling}
\usepackage{vwcol}
\usepackage{setspace}
\usepackage{empheq}
\usepackage{cancel}
\usepackage{esdiff}
\usepackage{multicol}
\usepackage{mdframed}
\usepackage{esdiff}
\usepackage{multicol}
\usepackage{tikz}
\usepackage{varwidth}

\intervalconfig {
	soft open fences
}

\newcommand{\alignedintertext}[1]{%
	\noalign{%
		\vskip\belowdisplayshortskip
		\vtop{\hsize=\linewidth#1\par
		\expandafter}%
		\expandafter\prevdepth\the\prevdepth
	}%
}

\renewcommand{\Re}{{\mathrm{Re}}}
\renewcommand{\Im}{{\mathrm{Im}}}

% \allowdisplaybreaks

%opening
\title{Problem Set \#52}
\author{Jayden Li}
\date{February 15, 2024}

\allowdisplaybreaks

\begin{document}
\setstretch{1.25}
\fontsize{12pt}{12pt}\selectfont
\setlength{\abovedisplayskip}{0pt}
\maketitle

\section*{Problem 5}

\begin{alignat*}{2}
	z_1&=0 &\qquad |z_1|&=0 \\
	z_2&=0^2+i=i & |z_2|&=1 \\
	z_3&=(-i)^2+i=-1+i & |z_3|&=\sqrt{2} \\
	z_4&=(-1+i)^2+i=-i & |z_4|&=1 \\
	z_5&=(-i)^2+i=-1+i & |z_5|&=\sqrt{2} \\
	z_6&=(-i+1)^2+i=-i & |z_6|&=1
\end{alignat*}

I claim that:
\begin{equation*}
	z_n=\begin{cases}
		0\quad n=1 \\
		1\quad\text{$n$ even} \\
		\sqrt{2}\quad\text{else}
	\end{cases}
\end{equation*}

Therefore \boxed{z_{111}=\sqrt{2}}

\section*{Problem 6}
Let $F=a+bi$ where $a,b\in\mathbb{R}$, $a>1$ and $0<b<1$.
\begin{align*}
	\frac{1}{F}&=\frac{1}{a+bi}\cdot\frac{a-bi}{a-bi} \\
	&=\frac{a-bi}{a+b} \\
	&=\frac{a}{a+b}+\left(-\frac{b}{a+b}\right)i
\end{align*}
Because $a,b<a+b$ and $a,b,(a+b)\in\mathbb{R}^+$, $0<\dfrac{a}{a+b}<1$ and $-1<-\dfrac{b}{a+b}<0$. \boxed{C} is the reciprocal of $F$.

\section*{Problem 7}
\begin{itemize}
\item[(a)]
	\begin{proof}	
		Let $z=a+bi$.
		\begin{align*}
			z\overline{z}&=(a+bi)(a-bi) \\
			&=a^2+b^2 \\
			&=\left(\sqrt{a^2+b^2}\right) \\
			&=|z|^2
		\end{align*}
	\end{proof}

\item[(b)]
	Let $z=a+bi$ and $w=c+di$.

	\centering
	\begin{minipage}[t]{0.4\linewidth}
		\begin{align*}
			|z|&=|w|=3 \\
			\sqrt{a^2+b^2}&=\sqrt{c^2+d^2}=3 \\
			a^2+b^2&=c^2+d^2=9 \\
			\\
			|z-w|&=|a+bi-c-di| \\
			&=\sqrt{(a-c)^2+(b-d)^2} \\
			&=\sqrt{a^2-2ac+c^2+b^2-2bd+d^2} \\
			&=\sqrt{9+9+14} \\
			&=\sqrt{32} \\
			&=\boxed{4\sqrt{2}}
		\end{align*}
	\end{minipage}
	\begin{minipage}[t]{0.4\linewidth}
		\begin{align*}
			|z+w|&=2 \\
			|a+bi+c+di|&=2 \\
			\sqrt{(a+c)^2+(b+d)^2}&=2 \\
			(a+c)^2+(b+d)^2&=4 \\
			a^2+2ac+c^2+b^2+2bd+d^2&=4 \\
			9+2ac+9+2bd&=4 \\
			2ac+2bd&=-14 \\
			-2ac-2bd&=14
		\end{align*}
	\end{minipage}

	\justifying

\end{itemize}

\section*{Problem 8}
Let $z=a+bi$.
\begin{itemize}
\item[(a)]
	\begin{align*}
		|z-3|&=|z+2i| \\
		|(a-3)+bi|&=|a+(b+2)i| \\
		\sqrt{(a-3)^2+b^2}&=\sqrt{a^2+(b+2)^2} \\
		\cancel{a^2}-6a+9+\cancel{b^2}&=\cancel{a^2}+\cancel{b^2}+4b+4 \\
		6a+4b&=5 \\
		b&=\frac{5-6a}{4}
	\end{align*}

\item[(b)]
	\begin{align*}
		z+|z|&=2+8i \\
		a+bi+\sqrt{a^2+b^2}&=2+8i \\
		\left(a+\sqrt{a^2+b^2}\right)+bi&=2+8i
	\end{align*}
	\begin{minipage}[t]{0.5\linewidth}
		\begin{align*}
			\Re\left(\left(a+\sqrt{a^2+b^2}\right)+bi\right)&=\Re(2+8i) \\
			a+\sqrt{a^2+8^2}&=2 \\
			(a-2)^2&=a^2+64 \\
			\cancel{a^2}-4a+4&=\cancel{a^2}+64 \\
			4a&=-60 \\
			a&=-15
		\end{align*}
	\end{minipage}
	\begin{minipage}[t]{0.5\linewidth}
		\begin{align*}
			\Im\left(\left(a+\sqrt{a^2+b^2}\right)+bi\right)&=\Im(2+8i) \\
			b&=8
		\end{align*}
		\begin{align*}
			|z|&=|-15+8i| \\
			|z|&=\sqrt{225+64} \\
			|z|&=\sqrt{289} \\
			\Aboxed{|z|&=17}
		\end{align*}
	\end{minipage}

	\centering
	\includegraphics*[width=0.8\linewidth]{q8b.png}

	\justifying

\end{itemize}

\section*{Problem 9}
Let $z=a+bi$.
\begin{align*}
	|z-4+5i|&=2\sqrt{3} \\
	|(a-4)+(b+5)i|&=2\sqrt{3} \\
	(a-4)^2+(b+5)^2&=\left(2\sqrt{3}\right)^2
	\intertext{Turn this from the complex plane to the real Cartesian plane by applying $a=x,b=y$.}
	(x-4)^2+(y+5)^2&=\left(2\sqrt{3}\right)^2
\end{align*}
This is the equation of a circle with radius $2\sqrt{3}$. The radius of this circle is:
\begin{equation*}
	\pi\left(2\sqrt{3}\right)^2=\boxed{12\pi}
\end{equation*}

\end{document}